checkpoint proving refinement for log example

src/Examples/ExMach/WeakestPre.v
@@ -332,48 +332,57 @@ Proof.
   iNext. wp_ret. by iApply "HΦ".
 Qed.
 
-Fixpoint ptr_iter (n: nat) (iters: nat) :=
-  (match iters with
-  | O => n d↦ 0
-  | S n' => n d↦ 0 ∗ (ptr_iter (S n) n')
-  end)%I.
+Section PtrIter.
+  Context (ptsto: nat -> nat -> iProp Σ).
+  Infix "g↦" := (ptsto) (at level 0).
 
-Fixpoint rep_delete n (mem: gmap addr nat) :=
-  match n with
-  | O => mem
-  | S n' => delete n' (rep_delete n' mem)
-  end.
+  Fixpoint ptr_iter (n: nat) (iters: nat) :=
+    (match iters with
+     | O => n g↦ 0
+     | S n' => n g↦ 0 ∗ (ptr_iter (S n) n')
+     end)%I.
 
-Lemma rep_delete_lookup m n:
-  m ≥ n → rep_delete n ExMach.init_zero !! m = ExMach.init_zero !! m.
-Proof.
-  intros ?. induction n.
-  * rewrite /rep_delete. auto.
-  * rewrite /rep_delete lookup_delete_ne; last lia. eapply IHn. lia.
-Qed.
+  Fixpoint rep_delete n (mem: gmap addr nat) :=
+    match n with
+    | O => mem
+    | S n' => delete n' (rep_delete n' mem)
+    end.
 
-Lemma disk_ptr_iter_split_aux n iters:
-  n + iters < size →
-  (([∗ map] i↦v ∈ rep_delete n ExMach.init_zero, i d↦ v)
-     -∗ ptr_iter n iters ∗ [∗ map] i↦v ∈ rep_delete (n + S iters) ExMach.init_zero, i d↦ v)%I.
-Proof.
-  revert n. induction iters.
-  - intros n ?. rewrite (big_opM_delete _ _ n 0); last first.
-    rewrite rep_delete_lookup.
-    { apply init_zero_lookup_lt_zero; first by lia. }
-    { auto. }
-    replace (n + 1) with (S n) by lia.
-    iIntros "(?&?)". iFrame.
-  - intros n ?.
-    rewrite (big_opM_delete _ _ n 0); last first.
-    rewrite rep_delete_lookup.
-    { apply init_zero_lookup_lt_zero; first by lia. }
-    { auto. }
-    replace (n + S (S iters)) with (S n + S iters) by lia.
-    iIntros "(?&?)". iFrame.
-    iApply IHiters; first by lia.
-    eauto.
-Qed.
+  Lemma rep_delete_lookup m n:
+    m ≥ n → rep_delete n ExMach.init_zero !! m = ExMach.init_zero !! m.
+  Proof.
+    intros ?. induction n.
+    * rewrite /rep_delete. auto.
+    * rewrite /rep_delete lookup_delete_ne; last lia. eapply IHn. lia.
+  Qed.
+
+  Lemma gen_ptr_iter_split_aux n iters:
+    n + iters < size →
+    (([∗ map] i↦v ∈ rep_delete n ExMach.init_zero, i g↦ v)
+       -∗ ptr_iter n iters ∗ [∗ map] i↦v ∈ rep_delete (n + S iters) ExMach.init_zero, i g↦ v)%I.
+  Proof.
+    revert n. induction iters.
+    - intros n ?. rewrite (big_opM_delete _ _ n 0); last first.
+      rewrite rep_delete_lookup.
+      { apply init_zero_lookup_lt_zero; first by lia. }
+      { auto. }
+      replace (n + 1) with (S n) by lia.
+      iIntros "(?&?)". iFrame.
+    - intros n ?.
+      rewrite (big_opM_delete _ _ n 0); last first.
+      rewrite rep_delete_lookup.
+      { apply init_zero_lookup_lt_zero; first by lia. }
+      { auto. }
+      replace (n + S (S iters)) with (S n + S iters) by lia.
+      iIntros "(?&?)". iFrame.
+      iApply IHiters; first by lia.
+      eauto.
+  Qed.
+
+End PtrIter.
+
+Definition disk_ptr_iter_split_aux := gen_ptr_iter_split_aux (fun l v => l d↦ v)%I.
+Definition mem_ptr_iter_split_aux := gen_ptr_iter_split_aux (fun l v => l m↦ v)%I.
 
 End lifting.
 
